src/FcEtt/ext_wf.v
@@ -16,14 +16,14 @@ Require Import FcEtt.toplevel.
    -- all components are locally closed in any judgement
   *)
 
-Lemma Path_lc : forall F a R, Path F a R -> lc_tm a.
+Lemma Path_lc : forall F a R, Path a F R -> lc_tm a.
 Proof. intros. induction H; eauto.
 Qed.
 
-Lemma uniq_Path : forall F F' a R, Path F a R -> Path F' a R -> F = F'.
+(* Lemma uniq_Path : forall F F' a R, Path a F R -> Path a F' R -> F = F'.
 Proof. intros. generalize dependent F'. induction H; intros; auto.
        inversion H0; auto.
-       inversion H1; subst. assert (Ax a A R1 = Cs A0).
+       inversion H1; subst. assert (Ax p a A R1 Rs = Cs A0).
        eapply binds_unique; eauto using uniq_toplevel. inversion H2.
        auto. inversion H1; subst. eauto.
        inversion H0; subst. eauto. 
@@ -34,13 +34,13 @@ Proof. intros; induction H; eauto using Path_lc.
 Qed.
 
 
-Hint Resolve Value_lc Path_lc : lc.
+Hint Resolve Value_lc Path_lc : lc. *)
 
 
 (* -------------------------------- *)
 
 Lemma ctx_wff_mutual :
-  (forall G0 a A R, Typing G0 a A R -> Ctx G0) /\
+  (forall G0 a A, Typing G0 a A -> Ctx G0) /\
   (forall G0 phi,   PropWff G0 phi -> Ctx G0) /\
   (forall G0 D p1 p2, Iso G0 D p1 p2 -> Ctx G0) /\
   (forall G0 D A B T R,   DefEq G0 D A B T R -> Ctx G0) /\
@@ -57,28 +57,39 @@ Definition DefEq_Ctx := fourth ctx_wff_mutual.
 
 Hint Resolve Typing_Ctx PropWff_Ctx Iso_Ctx DefEq_Ctx.
 
+Fixpoint ctx_nom (G : context) := match G with
+  | nil => nil
+  | (x, Tm _) :: G' => (x, Nom) :: ctx_nom G'
+  | (x, Co _) :: G' => ctx_nom G'
+  end.
+
 Lemma Ctx_uniq : forall G, Ctx G -> uniq G.
   induction G; try auto.
   inversion 1; subst; solve_uniq.
 Qed.
 
-Lemma dom_rctx_le_ctx : forall G, dom (ctx_to_rctx G) [<=] dom G.
+Lemma dom_rctx_le_ctx : forall G, dom (ctx_nom G) [<=] dom G.
 Proof. intros; induction G; simpl. fsetdec.
        destruct a, s. simpl. fsetdec. fsetdec.
 Qed.
 
-Lemma ctx_to_rctx_uniq : forall G, Ctx G -> uniq (ctx_to_rctx G).
+Lemma notin_ctx_rctx : forall x G, x `notin` (dom G) -> x `notin` dom (ctx_nom G).
+Proof. intros. induction G. auto. destruct a, s; simpl in *.
+       all : pose (P := H); apply notin_add_2 in P; fsetdec.
+Qed.
+
+Lemma ctx_to_rctx_uniq : forall G, Ctx G -> uniq (ctx_nom G).
 Proof. intros G. induction G; intros.
         - simpl; auto.
         - inversion H; subst; simpl. apply Ctx_uniq in H.
           apply IHG in H2. econstructor; eauto. 
-          assert (P : dom (ctx_to_rctx G) [<=] dom G). 
+          assert (P : dom (ctx_nom G) [<=] dom G). 
           { apply dom_rctx_le_ctx. } fsetdec.
           inversion H. apply IHG; auto.
 Qed.
 
-Lemma ctx_to_rctx_binds_tm : forall G x A R, binds x (Tm A R) G ->
-                                             binds x R (ctx_to_rctx G).
+Lemma ctx_to_rctx_binds_tm : forall G x A, binds x (Tm A) G ->
+                                             binds x Nom (ctx_nom G).
 Proof. intros G. induction G; intros; simpl; eauto.
        destruct a, s. apply binds_cons_1 in H. inversion H; eauto.
        inversion H0. inversion H2. subst. auto.
@@ -89,7 +100,7 @@ Qed.
 Hint Resolve Ctx_uniq.
 
 Lemma lc_mutual :
-  (forall G0 a A R, Typing G0 a A R -> lc_tm a /\ lc_tm A) /\
+  (forall G0 a A, Typing G0 a A -> lc_tm a /\ lc_tm A) /\
   (forall G0 phi , PropWff G0 phi -> lc_constraint phi) /\
   (forall G0 D p1 p2,  Iso G0 D p1 p2 -> lc_constraint p1 /\ lc_constraint p2) /\
   (forall G0 D A B T R, DefEq G0 D A B T R -> lc_tm A /\ lc_tm B /\ lc_tm T) /\
@@ -98,7 +109,7 @@ Proof.
   eapply typing_wff_iso_defeq_mutual. 
   all: pre; basic_solve_n 2.
   all: split_hyp.
-  all: lc_solve.  
+  all: lc_solve.
 Qed.
 
 Definition Typing_lc  := first lc_mutual.
@@ -107,11 +118,11 @@ Definition Iso_lc     := third lc_mutual.
 Definition DefEq_lc   := fourth lc_mutual.
 Definition Ctx_lc     := fifth lc_mutual.
 
-Lemma Typing_lc1 : forall G0 a A R, Typing G0 a A R -> lc_tm a.
+Lemma Typing_lc1 : forall G0 a A, Typing G0 a A -> lc_tm a.
 Proof.
   intros. apply (first lc_mutual) in H. destruct H. auto.
 Qed.
-Lemma Typing_lc2 : forall G0 a A R, Typing G0 a A R -> lc_tm A.
+Lemma Typing_lc2 : forall G0 a A, Typing G0 a A -> lc_tm A.
 Proof.
   intros. apply (first lc_mutual) in H. destruct H. auto.
 Qed.
